dw/DeepWeb/Free/Monad/Internal.v
@@ -3,8 +3,6 @@ Set Contextual Implicit.
 
 Require Import DeepWeb.Free.Monad.Free.
 
-(** * Internals *)
-
 (* If we can interpret the events of one such monad as computations in
     another, we can extend that interpretation to the whole monad. *)
 
