dw/DeepWeb/Test/Rand.v
@@ -1,8 +1,0 @@
-From Coq Require Extraction.
-Require Import DeepWeb.Test.Client.
-
-Parameter flip : IO bool.
-Parameter rand : nat -> IO nat.
-
-Extract Constant flip => "Random.bool".
-Extract Constant rand => "fun n () -> Random.int n".
